Veir/Parser/AttrParser.lean
@@ -161,6 +161,36 @@ def parseOptionalDenseArrayAttr : AttrParserM (Option DenseArrayAttr) := do
   parsePunctuation ">"
   return some (DenseArrayAttr.mk elementType values)
 
+def parseFastMathFlag : AttrParserM FastMathFlagsAttr := do
+  if (← parseOptionalKeyword "fast".toByteArray) then
+    return { fast := true, nnan := false, ninf := false, nsz := false }
+  else if (← parseOptionalKeyword "nnan".toByteArray) then
+    return { fast := false, nnan := true, ninf := false, nsz := false }
+  else if (← parseOptionalKeyword "ninf".toByteArray) then
+    return { fast := false, nnan := false, ninf := true, nsz := false }
+  else if (← parseOptionalKeyword "nsz".toByteArray) then
+    return { fast := false, nnan := false, ninf := false, nsz := true }
+  else if (← parseOptionalKeyword "none".toByteArray) then
+    return { fast := false, nnan := false, ninf := false, nsz := false }
+  else
+    return { fast := false, nnan := false, ninf := false, nsz := false }
+
+/--
+  Parse an optional fastmath flags attribute, if present.
+-/
+def parseFloatFastMathFlagsAttr : AttrParserM (Option FastMathFlagsAttr) := do
+  parsePunctuation "<"
+  let values ← parseList parseFastMathFlag
+  parsePunctuation ">"
+  let mut floatFastMathFlags := FastMathFlagsAttr.mk false false false false
+  for flag in values do
+    floatFastMathFlags := { floatFastMathFlags with
+      fast := floatFastMathFlags.fast || flag.fast,
+      nnan := floatFastMathFlags.nnan || flag.nnan,
+      ninf := floatFastMathFlags.ninf || flag.ninf,
+      nsz := floatFastMathFlags.nsz || flag.nsz }
+  return some floatFastMathFlags
+
 def isClosingBracket (kind : TokenKind) : Bool :=
   kind = .greater || kind = .rParen || kind = .rSquare || kind = .rBrace
 
@@ -260,6 +290,10 @@ partial def parseOptionalDialectAttr : AttrParserM (Option Attribute) := do
   let startPos ← getPos
   let dialectName ← parseOptionalPrefixedKeyword .hashIdent
   let some dialectName := dialectName | return none
+
+  if dialectName = "llvm.fastmath".toByteArray then do
+    return ← parseFloatFastMathFlagsAttr
+
   if !(← getThe AttrParserState).allowUnregisteredDialect then
     throwAt startPos s!"attribute is not registered. Consider using --allow-unregistered-dialect."
   parsePunctuation "<"
